$\displaystyle \mathbf{\int \frac{e^{2x}}{e^{x} + 3}\,dx}$
\nopagebreak
\begin{align*}
\text{Sustituyendo: } &u = e^{x} \;\;\Rightarrow\; du = e^{x}\,dx \\[6pt]
\text{Entonces } &e^{2x} = (e^{x})^{2} = u^{2}, \quad dx = \frac{du}{u}. \\[6pt]
\int \frac{e^{2x}}{e^{x} + 3}\,dx
&= \int \frac{u^{2}}{u + 3}\cdot \frac{du}{u} \\[6pt]
&= \int \frac{u}{u + 3}\,du \\[6pt]
\text{Dividiendo: } &\frac{u}{u + 3} = 1 - \frac{3}{u + 3}. \\[6pt]
\int \frac{e^{2x}}{e^{x} + 3}\,dx
&= \int \left(1 - \frac{3}{u + 3}\right)\,du \\[6pt]
&= \int 1\,du - 3\int \frac{1}{u + 3}\,du \\[6pt]
&= u - 3\ln|u + 3| + C
\end{align*}
\[
\boxed{\displaystyle 
\int \frac{e^{2x}}{e^{x} + 3}\,dx
= e^{x} - 3\ln\bigl(e^{x} + 3\bigr) + C.}
\]
