$\displaystyle \mathbf{\int \frac{2^{x+1} - 5^{x-1}}{10^{x}}\,dx}$
\nopagebreak
\begin{align*}
\text{Operando: } &2^{x+1} = 2\cdot 2^{x}, \quad 5^{x-1} = \frac{1}{5}\,5^{x}, \quad 10^{x}=2^{x}5^{x}. \\[6pt]
&\frac{2^{x+1} - 5^{x-1}}{10^{x}}
= \frac{2\cdot 2^{x}}{2^{x}5^{x}} - \frac{\tfrac{1}{5}\,5^{x}}{2^{x}5^{x}} \\[6pt]
&= 2\cdot 5^{-x} - \frac{1}{5}\,2^{-x}. \\[6pt]
\int \frac{2^{x+1} - 5^{x-1}}{10^{x}}\,dx
&= \int \left(2\cdot 5^{-x} - \frac{1}{5}\,2^{-x}\right)\,dx \\[6pt]
\text{Usando } &\int a^{-x}\,dx = -\frac{a^{-x}}{\ln a} + C, \\[6pt]
\int \left(2\cdot 5^{-x} - \frac{1}{5}\,2^{-x}\right)\,dx
&= 2\left(-\frac{5^{-x}}{\ln 5}\right) - \frac{1}{5}\left(-\frac{2^{-x}}{\ln 2}\right) + C \\[6pt]
&= -\frac{2}{\ln 5}\,5^{-x} + \frac{1}{5\ln 2}\,2^{-x} + C
\end{align*}
\[
\boxed{\displaystyle 
\int \frac{2^{x+1} - 5^{x-1}}{10^{x}}\,dx
= -\frac{2}{\ln 5}\,5^{-x} + \frac{1}{5\ln 2}\,2^{-x} + C.}
\]
