$\displaystyle \mathbf{\int \frac{9^{x} - 4^{x}}{2^{x}3^{x}}\,dx}$
\nopagebreak
\begin{align*}
\text{Operando: } &9^{x} = 3^{2x}, \quad 4^{x} = 2^{2x}, \quad 2^{x}3^{x}=6^{x}. \\[6pt]
&\frac{9^{x} - 4^{x}}{2^{x}3^{x}}
= \frac{3^{2x}}{2^{x}3^{x}} - \frac{2^{2x}}{2^{x}3^{x}} \\[6pt]
&= \left(\frac{3}{2}\right)^{x} - \left(\frac{2}{3}\right)^{x}. \\[6pt]
\int \frac{9^{x} - 4^{x}}{2^{x}3^{x}}\,dx
&= \int \left[\left(\frac{3}{2}\right)^{x} - \left(\frac{2}{3}\right)^{x}\right] dx \\[6pt]
\text{Usando } &\int a^{x}\,dx = \frac{a^{x}}{\ln a} + C, \\[6pt]
&= \frac{\left(\tfrac{3}{2}\right)^{x}}{\ln\!\left(\tfrac{3}{2}\right)} - \frac{\left(\tfrac{2}{3}\right)^{x}}{\ln\!\left(\tfrac{2}{3}\right)} + C
\end{align*}
\[
\boxed{\displaystyle 
\int \frac{9^{x} - 4^{x}}{2^{x}3^{x}}\,dx
= \frac{\left(\tfrac{3}{2}\right)^{x}}{\ln\!\left(\tfrac{3}{2}\right)} - \frac{\left(\tfrac{2}{3}\right)^{x}}{\ln\!\left(\tfrac{2}{3}\right)} + C}
\]
