$\displaystyle \mathbf{\int \sqrt{\frac{1-\sin x}{1+\sin x}}\,dx}$
\nopagebreak
\[
\text{Usamos la identidad: } \frac{1-\sin x}{1+\sin x} = \frac{\cos^2 x}{(1+\sin x)^2} = \left(\frac{\cos x}{1+\sin x}\right)^2
\]
\[
\text{Entonces } \sqrt{\frac{1-\sin x}{1+\sin x}} = \frac{\cos x}{1+\sin x}
\]
\[
\int \sqrt{\frac{1-\sin x}{1+\sin x}}\,dx = \int \frac{\cos x}{1+\sin x}\,dx
\]

\[
\text{Sustituimos } t = 1+\sin x \implies dt = \cos x\, dx
\]

\[
\int \frac{\cos x}{1+\sin x}\,dx = \int \frac{dt}{t} = \ln|t| + C
\]

\[
\boxed{\displaystyle 
\int \sqrt{\frac{1-\sin x}{1+\sin x}}\,dx = \ln|1+\sin x| + C
}
\]
