$\displaystyle \mathbf{\int \frac{dx}{x^{2}\sqrt{x^{2}-7}}}$

\nopagebreak
\begin{align*}
\text{Sustitución trigonométrica: } 
&x = \sqrt{7}\sec\theta, 
\quad dx = \sqrt{7}\sec\theta\tan\theta\,d\theta. \\[4pt]
\text{Entonces } 
&\sqrt{x^{2}-7} = \sqrt{7\tan^{2}\theta} = \sqrt{7}\tan\theta. \\[4pt]
\text{Sustituyendo: } 
&\int \frac{dx}{x^{2}\sqrt{x^{2}-7}}
= \int \frac{\sqrt{7}\sec\theta\tan\theta}
{7\sec^{2}\theta\sqrt{7}\tan\theta}\,d\theta
= \tfrac{1}{7}\int \cos\theta\,d\theta. \\[4pt]
\text{Integrando: } 
&\tfrac{1}{7}\int \cos\theta\,d\theta 
= \tfrac{1}{7}\sin\theta + C. \\[4pt]
\text{Del triángulo: } 
&\sin\theta = \frac{\sqrt{x^{2}-7}}{x}. \\[4pt]
\text{Sustituyendo de nuevo: } 
&I_{44} = \tfrac{1}{7}\frac{\sqrt{x^{2}-7}}{x} + C.
\end{align*}

$$
\boxed{\displaystyle 
I_{44} = \frac{\sqrt{x^{2}-7}}{7x} + C}
$$

