$\displaystyle \mathbf{\int \frac{\sqrt{9-x^{2}}}{x^{2}}\,dx}$

\nopagebreak
$$
\begin{aligned}
\text{Sustitución trigonométrica: } &
x = 3\sin\theta, \quad dx = 3\cos\theta\,d\theta. \\[4pt]
\text{Triángulo: } &
\text{hipotenusa } 3,\; \text{opuesto } x,\; \text{adyacente } \sqrt{9-x^{2}}. \\[6pt]
\text{Sustituyendo: } &
\frac{\sqrt{9-x^{2}}}{x^{2}}\,dx
= \frac{3\cos\theta}{9\sin^{2}\theta}\cdot 3\cos\theta\,d\theta
= \cot^{2}\theta\,d\theta. \\[6pt]
\text{Integramos: } &
\int \cot^{2}\theta\,d\theta
= \int (\csc^{2}\theta - 1)\,d\theta
= -\cot\theta - \theta + C. \\[6pt]
\text{Regresando a } x: &
\cot\theta = \frac{\sqrt{9-x^{2}}}{x}, \quad 
\theta = \arcsin\!\left(\frac{x}{3}\right). \\[4pt]
\Rightarrow &
\int \frac{\sqrt{9-x^{2}}}{x^{2}}\,dx
= -\frac{\sqrt{9-x^{2}}}{x} - \arcsin\!\left(\frac{x}{3}\right) + C.
\end{aligned}
$$

$$
\boxed{\displaystyle 
I_{45} = -\frac{\sqrt{9-x^{2}}}{x} - \arcsin\!\left(\frac{x}{3}\right) + C}
$$
