$\displaystyle \mathbf{\int \frac{dx}{(5 - 4x - x^{2})^{3/2}}}$

\nopagebreak
$$
\begin{aligned}
&5 - 4x - x^{2} = 9 - (x + 2)^{2}. \\[4pt]
\text{Sea } &u = x + 2 \;\Rightarrow\; du = dx. \\[4pt]
\text{Sustitución trigonométrica: } &u = 3\sin\theta,\quad du = 3\cos\theta\,d\theta. \\[4pt]
\text{Entonces: } &(9 - u^{2}) = 9\cos^{2}\theta. \\[4pt]
\Rightarrow\;
\frac{du}{(9 - u^{2})^{3/2}}
= \frac{3\cos\theta}{(3\cos\theta)^{3}}\,d\theta
= \frac{1}{9}\sec^{2}\theta\,d\theta. \\[6pt]
\text{Integramos: } &
\int \frac{du}{(9 - u^{2})^{3/2}}
= \frac{1}{9}\int \sec^{2}\theta\,d\theta
= \frac{1}{9}\tan\theta + C. \\[6pt]
\text{Volviendo a } x: &
\tan\theta = \frac{u}{\sqrt{9 - u^{2}}}
= \frac{x + 2}{\sqrt{5 - 4x - x^{2}}}. \\[6pt]
\boxed{\displaystyle
I_{47} = \frac{x + 2}{9\sqrt{5 - 4x - x^{2}}} + C.}
\end{aligned}
$$
