$\displaystyle \mathbf{\int x\sqrt{x^{4}+2x^{2}-1}\,dx}$

\nopagebreak
$$
\text{Sea } u = x^{2} \Rightarrow du = 2x\,dx \Rightarrow x\,dx = \tfrac{1}{2}du.
$$
$$
\Rightarrow\; \int x\sqrt{x^{4}+2x^{2}-1}\,dx
= \tfrac{1}{2}\int \sqrt{u^{2}+2u-1}\,du.
$$
$$
\text{Completamos el cuadrado: } u^{2}+2u-1 = (u+1)^{2} - 2.
$$
$$
\text{Sea } v = u + 1 \Rightarrow dv = du.
$$
$$
\Rightarrow\; \tfrac{1}{2}\int \sqrt{v^{2}-2}\,dv.
$$
$$
\text{Usamos la f√≥rmula: } 
\int \sqrt{v^{2}-a^{2}}\,dv
= \tfrac{1}{2}\big(v\sqrt{v^{2}-a^{2}} - a^{2}\ln|v+\sqrt{v^{2}-a^{2}}|\big) + C.
$$
$$
\text{Aplicando con } a^{2}=2:
\quad \tfrac{1}{4}\big(v\sqrt{v^{2}-2} - 2\ln|v+\sqrt{v^{2}-2}|\big) + C.
$$
$$
\text{Regresando a } x: \quad v = u + 1 = x^{2} + 1.
$$
$$
\boxed{
I_{48} =
\tfrac{1}{4}\Big[(x^{2}+1)\sqrt{x^{4}+2x^{2}-1}
- \sqrt{2}\,\ln\!\big|x^{2}+1+\sqrt{x^{4}+2x^{2}-1}\big|\Big] + C.
}
$$
