$\displaystyle \mathbf{\int \frac{6x^{2} - 2x - 1}{4x^{3} - x}\,dx}$

\nopagebreak
\[
\text{Factorizamos el denominador:}
\]
\[
4x^{3} - x = x(2x - 1)(2x + 1)
\]

\[
\text{Planteamos fracciones parciales:}
\]
\[
\frac{6x^{2} - 2x - 1}{x(2x - 1)(2x + 1)}
= \frac{A}{x} + \frac{B}{2x - 1} + \frac{C}{2x + 1}
\]

\[
\text{Multiplicamos por el denominador común y comparamos coeficientes:}
\]
\[
6x^{2} - 2x - 1 = A(2x - 1)(2x + 1) + Bx(2x + 1) + Cx(2x - 1)
\]

\[
A = 1, \quad B = -\tfrac{1}{4}, \quad C = \tfrac{3}{4}
\]

\[
\text{Sustituyendo en la integral:}
\]
\[
\int \frac{6x^{2} - 2x - 1}{4x^{3} - x}\,dx
= \int\!\left(\frac{1}{x} - \frac{1}{4(2x - 1)} + \frac{3}{4(2x + 1)}\right)dx
\]

\[
\text{Integrando término a término:}
\]
\[
I_{51}
= \ln|x| - \tfrac{1}{4}\ln|2x - 1| + \tfrac{3}{4}\ln|2x + 1| + C
\]

\[
\boxed{\displaystyle
I_{51}
= \frac{3}{4}\ln|2x + 1|
- \frac{1}{4}\ln|2x - 1|
+ \ln|x| + C
}
\]
