$\displaystyle \mathbf{\int \frac{2x^{2}-5}{x^{4}-5x^{2}+6}\,dx}$

\nopagebreak
$$
\begin{aligned}
\text{Operando: } &
\text{Factorizamos el denominador: } \\[4pt]
&x^{4}-5x^{2}+6=(x^{2}-2)(x^{2}-3). \\[6pt]
\text{Buscamos una descomposición: } &
\frac{2x^{2}-5}{(x^{2}-2)(x^{2}-3)}
= \frac{A}{x^{2}-2} + \frac{B}{x^{2}-3}. \\[6pt]
\text{Multiplicando por }(x^{2}-2)(x^{2}-3): &
2x^{2}-5 = A(x^{2}-3) + B(x^{2}-2). \\[6pt]
\text{Igualando coeficientes: } &
(A+B)x^{2} + (-3A-2B) = 2x^{2}-5. \\[4pt]
\text{De donde: } &A+B=2,\quad -3A-2B=-5. \\[4pt]
\text{Resolviendo: } &A=1,\; B=1. \\[8pt]
\text{Por tanto: } &
\frac{2x^{2}-5}{x^{4}-5x^{2}+6}
= \frac{1}{x^{2}-2} + \frac{1}{x^{2}-3}. \\[8pt]
\text{Integramos término a término: } &
\int \frac{dx}{x^{2}-a}
= \frac{1}{2\sqrt{a}}\ln\!\left|\frac{x-\sqrt{a}}{x+\sqrt{a}}\right| + C.
\\[6pt]
\text{Aplicando con } a=2 \text{ y } a=3: &\\[4pt]
\int \frac{1}{x^{2}-2}\,dx
&= \frac{1}{2\sqrt{2}}\ln\!\left|\frac{x-\sqrt{2}}{x+\sqrt{2}}\right|, \\[4pt]
\int \frac{1}{x^{2}-3}\,dx
&= \frac{1}{2\sqrt{3}}\ln\!\left|\frac{x-\sqrt{3}}{x+\sqrt{3}}\right|.
\end{aligned}
$$

$$
\boxed{\displaystyle 
\int \frac{2x^{2}-5}{x^{4}-5x^{2}+6}\,dx
= \frac{1}{2\sqrt{3}}\ln\!\left|\frac{x-\sqrt{3}}{x+\sqrt{3}}\right|
+ \frac{1}{2\sqrt{2}}\ln\!\left|\frac{x-\sqrt{2}}{x+\sqrt{2}}\right| + C}
$$
