$\displaystyle \mathbf{\int \frac{2x^{2} - 3x - 2}{x^{3} + x^{2} - 2x}\,dx}$

\nopagebreak
\[
\text{Factorizamos el denominador:}
\]
\[
x^{3} + x^{2} - 2x = x(x - 1)(x + 2)
\]

\[
\text{Planteamos fracciones parciales:}
\]
\[
\frac{2x^{2} - 3x - 2}{x(x - 1)(x + 2)}
= \frac{A}{x} + \frac{B}{x - 1} + \frac{C}{x + 2}
\]

\[
\text{Multiplicamos por el denominador común y comparamos coeficientes:}
\]
\[
2x^{2} - 3x - 2 = A(x - 1)(x + 2) + B x(x + 2) + C x(x - 1)
\]

\[
A = 2, \quad B = -1, \quad C = 1
\]

\[
\text{Sustituyendo en la integral:}
\]
\[
\int \frac{2x^{2} - 3x - 2}{x^{3} + x^{2} - 2x}\,dx
= \int\!\left(\frac{2}{x} - \frac{1}{x - 1} + \frac{1}{x + 2}\right)dx
\]

\[
\text{Integrando término a término:}
\]
\[
I_{53} = 2\ln|x| - \ln|x - 1| + \ln|x + 2| + C
\]

\[
\boxed{\displaystyle
I_{53} = 2\ln|x + 2| + \ln|x| - \ln|x - 1| + C
}
\]
