$\displaystyle \mathbf{\int \frac{x^{2}}{(x^{2}+2x+2)^{2}}\,dx}$

\nopagebreak
\text{Operando: Completamos el cuadrado del denominador:}

$$
x^{2}+2x+2 = (x+1)^{2}+1.
$$

\nopagebreak
\text{Sustituimos } u = x+1, \ du = dx, \ x = u-1:

$$
\int \frac{x^{2}}{(x^{2}+2x+2)^{2}}\,dx
= \int \frac{(u-1)^{2}}{(u^{2}+1)^{2}}\,du
= \int \frac{u^{2}-2u+1}{(u^{2}+1)^{2}}\,du.
$$

\nopagebreak
\text{Separamos la integral:}

$$
\int \frac{u^{2}-2u+1}{(u^{2}+1)^{2}}\,du
= \int \frac{u^{2}+1}{(u^{2}+1)^{2}}\,du - 2\int \frac{u}{(u^{2}+1)^{2}}\,du
= \int \frac{1}{u^{2}+1}\,du - 2\int \frac{u}{(u^{2}+1)^{2}}\,du.
$$

\nopagebreak
\text{Integramos cada t√©rmino:}

$$
\int \frac{1}{u^{2}+1}\,du = \arctan(u), \quad
\int \frac{u}{(u^{2}+1)^{2}}\,du = \frac{-1}{2(u^{2}+1)}.
$$

\nopagebreak
\text{Por tanto:}

$$
\int \frac{x^{2}}{(x^{2}+2x+2)^{2}}\,dx
= \arctan(u) + \frac{1}{u^{2}+1} + C
= \arctan(x+1) + \frac{1}{x^{2}+2x+2} + C.
$$

\nopagebreak
\[
\boxed{\displaystyle
\int \frac{x^{2}}{(x^{2}+2x+2)^{2}}\,dx
= \arctan(x+1) + \frac{1}{x^{2}+2x+2} + C}
\]
