$\displaystyle \mathbf{\int \frac{1}{x^{5}+x^{4}-2x^{3}-2x^{2}+x+1}\,dx}$

\nopagebreak
\[
\textbf{Desarrollo:}
\]
\[
\begin{aligned}
x^{5}+x^{4}-2x^{3}-2x^{2}+x+1
&= (x^{5}+x^{4}) + (-2x^{3}-2x^{2}) + (x+1) \\[2pt]
&= x^{4}(x+1) - 2x^{2}(x+1) + (x+1) \\[2pt]
&= (x+1)(x^{4}-2x^{2}+1) \\[2pt]
&= (x+1)(x^{2}-1)^{2} = (x+1)^{3}(x-1)^{2}.
\end{aligned}
\]

\nopagebreak
\[
\textbf{Descomposición en fracciones parciales:}
\]
\[
\frac{1}{(x+1)^{3}(x-1)^{2}}
= \frac{A}{x+1} + \frac{B}{(x+1)^{2}} + \frac{C}{(x+1)^{3}}
+ \frac{D}{x-1} + \frac{E}{(x-1)^{2}},
\]
con:
\[
A=\tfrac{3}{16}, \quad B=-\tfrac{1}{4}, \quad C=-\tfrac{1}{8}, \quad
D=-\tfrac{1}{8}, \quad E=-\tfrac{3}{16}.
\]

\nopagebreak
\[
\textbf{Integrando término a término:}
\]
\[
\begin{aligned}
\int \frac{A}{x+1}\,dx &= A\ln|x+1|, &
\int \frac{B}{(x+1)^{2}}\,dx &= -\frac{B}{x+1}, \\[4pt]
\int \frac{C}{(x+1)^{3}}\,dx &= -\frac{C}{2(x+1)^{2}}, &
\int \frac{D}{x-1}\,dx &= D\ln|x-1|, \\[4pt]
\int \frac{E}{(x-1)^{2}}\,dx &= -\frac{E}{x-1}.
\end{aligned}
\]

\nopagebreak
\[
\textbf{Por lo tanto:}
\]
\[
\boxed{%
\begin{gathered}
\displaystyle
\int \frac{1}{x^{5}+x^{4}-2x^{3}-2x^{2}+x+1}\,dx
= \frac{3}{16}\ln|x+1|
- \frac{1}{4(x+1)} \\[4pt]
\displaystyle
- \frac{1}{8(x+1)^{2}}
- \frac{1}{8(x-1)}
- \frac{3}{16}\ln|x-1|
+ C
\end{gathered}
}
\]
