$
\displaystyle \mathbf{\int \operatorname{arccot}\!\big(\sqrt{x}\,\big)\,dx}
$

\nopagebreak
\begin{align*}
\text{Operando: } 
&\text{Hacemos la sustitución: } t=\sqrt{x}\ (\Rightarrow x=t^{2}), \\[4pt]
&dx=2t\,dt,\quad t\ge0. \\[6pt]
\text{Entonces: } 
&\int \operatorname{arccot}\!\big(\sqrt{x}\,\big)\,dx
= \int \operatorname{arccot}(t)\cdot 2t\,dt \\[4pt]
&= 2\int t\,\operatorname{arccot}(t)\,dt. \\[8pt]
\text{Aplicamos integración por partes: } 
&\int u\,dv = uv - \int v\,du. \\[6pt]
\text{Sea } 
&u=\operatorname{arccot}(t), \quad dv=2t\,dt. \\[6pt]
\text{Entonces: } 
&du = -\frac{1}{1+t^{2}}\,dt, \quad v=\int 2t\,dt = t^{2}. \\[6pt]
\text{Sustituyendo: } \\[4pt]
2\int t\,\operatorname{arccot}(t)\,dt
&= u v - \int v\,du \\[4pt]
&= t^{2}\operatorname{arccot}(t)
- \int t^{2}\!\left(-\frac{1}{1+t^{2}}\right)\!dt \\[4pt]
&= t^{2}\operatorname{arccot}(t)
+ \int \frac{t^{2}}{1+t^{2}}\,dt. \\[6pt]
\text{Observa que: } 
&\dfrac{t^{2}}{1+t^{2}} = 1 - \dfrac{1}{1+t^{2}}. \\[6pt]
\text{Por tanto: } \\[4pt]
2\int t\,\operatorname{arccot}(t)\,dt
&= t^{2}\operatorname{arccot}(t)
+ \int\!\left(1 - \frac{1}{1+t^{2}}\right)\!dt \\[4pt]
&= t^{2}\operatorname{arccot}(t)
+ t - \arctan(t) + C. \\[8pt]
\text{Regresando a } x\ (t=\sqrt{x}): \\[6pt]
\int \operatorname{arccot}\!\big(\sqrt{x}\,\big)\,dx
&= x\,\operatorname{arccot}\!\big(\sqrt{x}\,\big)
+ \sqrt{x} - \arctan\!\big(\sqrt{x}\,\big) + C.
\end{align*}

$$
\boxed{\displaystyle 
\int \operatorname{arccot}\!\big(\sqrt{x}\,\big)\,dx
= x\,\operatorname{arccot}\!\big(\sqrt{x}\,\big)
+ \sqrt{x} - \arctan\!\big(\sqrt{x}\,\big) + C}
$$

\nopagebreak
\begin{align*}
\text{Forma equivalente (usando } 
\arctan t=\tfrac{\pi}{2}-\operatorname{arccot} t,\ t\ge0\text{):} \\[6pt]
x\,\operatorname{arccot}\!\big(\sqrt{x}\,\big)
+ \sqrt{x} - \arctan\!\big(\sqrt{x}\,\big)
&= x\,\operatorname{arccot}t + t + \big(\operatorname{arccot}t - \tfrac{\pi}{2}\big) + C \\[4pt]
&= (x+1)\operatorname{arccot}\!\big(\sqrt{x}\,\big) + \sqrt{x} + C'.
\end{align*}

$$
\boxed{\displaystyle 
\int \operatorname{arccot}\!\big(\sqrt{x}\,\big)\,dx
= (x+1)\operatorname{arccot}\!\big(\sqrt{x}\,\big)
+ \sqrt{x} + C}
$$
