$\displaystyle \mathbf{\int x^{3}\mathrm{e}^{x^{2}}\,dx}$

\nopagebreak
\[
\text{Observamos que la derivada de } x^{2} \text{ es } 2x.
\]

\[
\text{Reescribimos el integrando: } 
x^{3}\mathrm{e}^{x^{2}} = x^{2}\cdot x\,\mathrm{e}^{x^{2}}.
\]

\[
\text{Sea } u = x^{2}, \quad du = 2x\,dx \Rightarrow x\,dx = \tfrac{1}{2}\,du.
\]

\[
\Rightarrow\quad
\int x^{3}\mathrm{e}^{x^{2}}\,dx 
= \tfrac{1}{2}\int u\,\mathrm{e}^{u}\,du.
\]

\[
\text{Aplicamos integraci√≥n por partes: } 
\int u\,dv = uv - \int v\,du,
\quad dv = \mathrm{e}^{u}\,du \Rightarrow v = \mathrm{e}^{u}.
\]

\[
\Rightarrow\quad
\int u\,\mathrm{e}^{u}\,du = u\,\mathrm{e}^{u} - \mathrm{e}^{u} + C.
\]

\[
\text{Sustituyendo:}\quad
\tfrac{1}{2}\int u\,\mathrm{e}^{u}\,du
= \tfrac{1}{2}\big(u\,\mathrm{e}^{u} - \mathrm{e}^{u}\big) + C.
\]

\[
\text{Regresando a la variable original } (u = x^{2}):
\quad
\int x^{3}\mathrm{e}^{x^{2}}\,dx
= \tfrac{1}{2}\,\mathrm{e}^{x^{2}}\,(x^{2} - 1) + C.
\]

\[
\boxed{
\displaystyle 
\int x^{3}\mathrm{e}^{x^{2}}\,dx
= \tfrac{1}{2}\,\mathrm{e}^{x^{2}}\,(x^{2} - 1) + C
}
\]
