$\displaystyle \mathbf{\int x^{3} \sqrt{x+1}\,dx}$

\nopagebreak
$$
\begin{aligned}
\text{Operando: } &
\text{Sea } u = x + 1 \implies du = dx, \; x = u - 1. \\[6pt]
&\text{Entonces } x^{3} = (u - 1)^{3}, \ \sqrt{x+1} = \sqrt{u}. \\[6pt]
\text{Sustituyendo: } &
\int x^{3}\sqrt{x+1}\,dx
= \int (u-1)^{3}u^{1/2}\,du \\[6pt]
&= \int (u^{7/2} - 3u^{5/2} + 3u^{3/2} - u^{1/2})\,du. \\[6pt]
\text{Integrando término a término: } &
\int u^{7/2}\,du = \tfrac{2}{9}u^{9/2}, \quad
\int u^{5/2}\,du = \tfrac{2}{7}u^{7/2}, \\[3pt]
&\int u^{3/2}\,du = \tfrac{2}{5}u^{5/2}, \quad
\int u^{1/2}\,du = \tfrac{2}{3}u^{3/2}. \\[6pt]
\Rightarrow\quad
\int x^{3}\sqrt{x+1}\,dx
&= \tfrac{2}{9}u^{9/2}
- \tfrac{6}{7}u^{7/2}
+ \tfrac{6}{5}u^{5/2}
- \tfrac{2}{3}u^{3/2} + C. \\[8pt]
\text{Volviendo a } x: &
u = x + 1. \\[6pt]
\Rightarrow\quad
\int x^{3}\sqrt{x+1}\,dx
&= \tfrac{2}{9}(x+1)^{9/2}
\\[3pt]
&\quad - \tfrac{6}{7}(x+1)^{7/2}
+ \tfrac{6}{5}(x+1)^{5/2}
- \tfrac{2}{3}(x+1)^{3/2} + C.
\end{aligned}
$$
