$\displaystyle \mathbf{\int x \cdot \frac{\ln\left(x + \sqrt{1 + x^{2}}\right)}{\sqrt{1 + x^{2}}}\,dx}$

\nopagebreak
$$
\begin{aligned}
\text{Observamos: } &
\frac{d}{dx}\sqrt{1+x^{2}}=\frac{x}{\sqrt{1+x^{2}}}. \\[6pt]
&\text{Sugerimos la sustituci칩n hiperb칩lica } x=\sinh t. \\[4pt]
&\text{Entonces } dx=\cosh t\,dt,\quad \sqrt{1+x^{2}}=\cosh t. \\[6pt]
&\text{Adem치s } \ln\big(x+\sqrt{1+x^{2}}\big)
= \ln(\sinh t+\cosh t)=\ln(e^{t})=t. \\[8pt]
\text{La integral queda: } &
\int x\cdot\frac{\ln(x+\sqrt{1+x^{2}})}{\sqrt{1+x^{2}}}\,dx
= \int t\cdot\sinh t\,dt. \\[10pt]
\text{Aplicamos integraci칩n por partes: } &
\int u\,dv = uv - \int v\,du. \\[6pt]
\text{Elegimos: } &
u=t,\quad dv=\sinh t\,dt. \\[4pt]
\text{Entonces: } &
du=dt,\quad v=\cosh t. \\[6pt]
\text{Luego: } &
\int t\sinh t\,dt = t\cosh t - \int \cosh t\,dt
= t\cosh t - \sinh t + C. \\[10pt]
\text{Volviendo a } x: &
t=\operatorname{arsinh}(x),\ \sinh t = x,\ \cosh t=\sqrt{1+x^{2}}. \\[6pt]
\Rightarrow\quad &
\int x\cdot\frac{\ln(x+\sqrt{1+x^{2}})}{\sqrt{1+x^{2}}}\,dx
= \sqrt{1+x^{2}}\,\operatorname{arsinh}(x) - x + C.
\end{aligned}
$$

$$
\boxed{\displaystyle
\int x\cdot\frac{\ln(x+\sqrt{1+x^{2}})}{\sqrt{1+x^{2}}}\,dx
= \sqrt{1+x^{2}}\,\operatorname{arsinh}(x) - x + C
}
$$
