$\displaystyle \mathbf{\int \frac{\ln(\sin x)}{\cos^{2} x}\,dx}$
\nopagebreak
\begin{align*}
    &\text{Sustituimos } t = \tan x \implies dt = \frac{dx}{\cos^2 x}, \\[2pt]
    &\text{entonces la integral se convierte en: } 
    \int \frac{\ln(\sin x)}{\cos^2 x}\,dx = \int \ln(\sin x)\, dt, \\[2pt]
    &\text{y usamos } \sin x = \frac{t}{\sqrt{1+t^2}} \implies \ln(\sin x) = \ln t - \frac{1}{2} \ln(1+t^2), \\[2pt]
    &\text{entonces: } \int \ln(\sin x)\, dt = \int \ln t\, dt - \frac{1}{2} \int \ln(1+t^2)\, dt.
\end{align*}

\[
\text{Sabemos que } \int \ln t\, dt = t \ln t - t, \quad \int \ln(1+t^2)\, dt = t \ln(1+t^2) - 2t + 2\arctan t
\]

\begin{align*}
    \int \frac{\ln(\sin x)}{\cos^2 x}\,dx 
    &= \big(t \ln t - t\big) - \frac{1}{2}\big(t \ln(1+t^2) - 2t + 2\arctan t\big) + C \\[2pt]
    &= t \ln t - \frac{1}{2} t \ln(1+t^2) - \arctan t + C \\[2pt]
    &= \tan x \ln(\tan x) - \frac{1}{2} \tan x \ln(1+\tan^2 x) - x + C \\[2pt]
    &= \tan x \ln(\tan x) - \tan x \ln(\sec x) - x + C \\[2pt]
    &= \tan x \ln(\sin x) - x + C
\end{align*}

\[
\boxed{\displaystyle 
\int \frac{\ln(\sin x)}{\cos^{2} x}\,dx = \tan x \ln(\sin x) - x + C
}
\]
