$\displaystyle \mathbf{ \int 
        \frac{x\,dx}{2 + \sqrt{1 + x}}
    }$ 
\nopagebreak
\begin{align*}
\text{Sustituyendo: } u &= \sqrt{x + 1} + 2\\[6pt]
du &= \frac{1}{2 \sqrt{x + 1}}\, dx\\[6pt]
x &= \left(u - 2\right)^{2} - 1\\[6pt]
\int \frac{x\,dx}{2 + \sqrt{1 + x}}
&= 2 \int \frac{\left(\left(u - 2\right)^{2} - 1\right) \left(u - 2\right)}{u} \, du\\[6pt]
&= 2\int u^{2} - 6u - \frac{6}{u} + 11\, du \\[6pt]
&= -12 \ln u + \frac{2u^{3}}{3} - 6u^{2} + 22u\\[6pt]
&= -12 \ln\left(\sqrt{x + 1} + 2\right) + \frac{2 \left(\sqrt{x + 1} + 2\right)^{3}}{3} - 6 \left(\sqrt{x + 1} + 2\right)^{2}\\[6pt]
&\;\;\;\; + 22 \left(\sqrt{x + 1} + 2\right) + C\\[6pt]
&= \frac{2 \left(-18 \ln\left(\sqrt{x + 1} + 2\right) + \sqrt{x + 1} \left(x + 10\right) - 3x\right)}{3} + C\\[6pt]
\end{align*}
\[
\boxed{\displaystyle \int
    \frac{x\,dx}{2 + \sqrt{1 + x}} 
    = = \frac{2 \left(-18 \ln\left(\sqrt{x + 1} + 2\right) + \sqrt{x + 1} \left(x + 10\right) - 3x\right)}{3} + C
}
\]  