$\displaystyle \mathbf{\int \left(x + \frac{1}{x}\right)^{\frac{3}{2}} \left(1 - \frac{1}{x^2}\right) \, dx}$
\nopagebreak
\begin{align*}
\text{Sustituyendo: } &u = x + \frac{1}{x} \\
&\Rightarrow du = \left(1 - \frac{1}{x^2}\right) dx \\
&\Rightarrow \left(1 - \frac{1}{x^2}\right) dx = du. \\[6pt]
\int \left(x + \frac{1}{x}\right)^{\frac{3}{2}} \left(1 - \frac{1}{x^2}\right) \, dx
&= \int u^{\frac{3}{2}} \, du \\[6pt]
&= \frac{u^{\frac{5}{2}}}{\frac{5}{2}} + C \\[6pt]
&= \frac{2}{5} u^{\frac{5}{2}} + C \\[6pt]
&= \frac{2}{5} \left(x + \frac{1}{x}\right)^{\frac{5}{2}} + C
\end{align*}
\[
\boxed{\displaystyle \int 
\left(x + \frac{1}{x}\right)^{\frac{3}{2}} \left(1 - \frac{1}{x^2}\right) \, dx 
= \frac{2}{5} \left(x + \frac{1}{x}\right)^{\frac{5}{2}} + C
}
\]
