$\displaystyle \mathbf{\int \frac{x^{3} - 4x^{2} + 5x - 1}{x^{2} - 2x + 1} \, dx}$
\nopagebreak
\begin{align*}
\intertext{Dividiendo:} \\[4pt]
\int \frac{x^{3} - 4x^{2} + 5x - 1}{x^{2} - 2x + 1} \, dx
&= \int \left(\frac{1}{x^{2} - 2x + 1} + x - 2\right) dx\\[6pt]
&= \int \frac{1}{x^{2} - 2x + 1} \, dx + \int x \, dx - 2 \int \, dx\\[6pt]
\text{Resolviendo: }&\int \frac{1}{x^{2} - 2x + 1} \, dx \\[6pt]
&\int \frac{1}{\left(x - 1\right)^{2}} \, dx\\[6pt]
\text{Sustituyendo: } &u = x - 1 
\;\;\Rightarrow\; du = dx \\[6pt]
\int \frac{1}{\left(x - 1\right)^{2}} \, dx
&= \int \frac{1}{u^{2}} \, du\\[6pt]
&= -\frac{1}{u}\\[6pt]
&= -\frac{1}{x - 1}\\[6pt]
\text{Reemplazando}\\[6pt]
\int \frac{1}{x^{2} - 2x + 1} \, dx + \int x \, dx - 2 \int dx\\[6pt]
&= -\frac{1}{x - 1} + \int x \, dx - 2 \int dx\\[6pt]
&= -\frac{1}{x - 1} + \frac{x^{2}}{2} - 2x  + C
\end{align*}
\[
\boxed{\displaystyle 
\int \frac{x^{3} - 4x^{2} + 5x - 1}{x^{2} - 2x + 1} \, dx
= \frac{x^{2}}{2} - 2x - \frac{1}{x - 1} + C
}
\]
