$\displaystyle \mathbf{ \int 
       \sqrt{x + 3} \left(x + 1\right)^{2} 
    \,dx}$ 
\nopagebreak
\begin{align*}
\text{Sustituyendo: } &u = x + 3 
\;\;\Rightarrow\; du = dx \\[6pt]
\int \sqrt{x + 3} \left(x + 1\right)^{2} \,dx
&= \int \left(u - 2\right)^{2} \sqrt{u} \, du \\[6pt]
&= \int u^{\frac{5}{2}} - 4u^{\frac{3}{2}} + 4 \sqrt{u}du\\[6pt]
&= \frac{2u^{\frac{7}{2}}}{7} - \frac{8u^{\frac{5}{2}}}{5} + \frac{8u^{\frac{3}{2}}}{3}\\[6pt]
&= \frac{2 \left(x + 3\right)^{\frac{7}{2}}}{7}
- \frac{8 \left(x + 3\right)^{\frac{5}{2}}}{5} 
+ \frac{8 \left(x + 3\right)^{\frac{3}{2}}}{3} + C\\[6pt]
\text{Simplificando: }&= \frac{2 \left(x + 3\right)^{\frac{3}{2}} \left(15x^{2} + 6x + 23\right)}{105} + C\\[6pt]
\end{align*}
\[
\boxed{\displaystyle 
\int \left(x + 1\right)^{2} \sqrt{x + 3}\,dx 
= \frac{\left(x + 3\right)^{\frac{3}{2}} \left(30x^{2} + 12x + 46\right)}{105} + C
}
\]