$\displaystyle \mathbf{ \int 
        \frac{2x^{3}}{x^{2} - 4}
    \,dx}$ 

\begin{align*}
\text{Sustituyendo: } &u = x^{2} - 4 
\;\;\Rightarrow\; du = 2x\,dx\\[6pt]
\int \frac{2x^{3}}{x^{2} - 4}\,dx
&= \, \int \frac{u + 4}{u} \, du \\[6pt]
&= \int 1 + \frac{4}{u}du \\[6pt]
&= u + 4 \ln\left(u\right)\\[6pt]
&= x^{2} - 4 + 4 \ln\left(\left|x^{2} - 4\right|\right) + C\\[6pt]
&= 4 \ln\left(\left|x^{2} - 4\right|\right) + x^{2} + C
\end{align*}
\[
\boxed{\displaystyle 
    \int \frac{2x^{3}}{x^{2} - 4}\,dx 
    = 4 \ln\left(\left|x^{2} - 4\right|\right) + x^{2} + C
}
\]