$\displaystyle \mathbf{ \int 
        \frac{e^{x} - 1}{e^{x} + 1}
    \,dx}$ 
\nopagebreak
\begin{align*}
\int \frac{e^{x} - 1}{e^{x} + 1}\, dx
&= \int \left(\frac{e^{x} + 1}{e^{x} + 1} - \frac{2}{e^{x} + 1}\right) dx \\[6pt]
&= \int 1 - \frac{2}{e^{x} + 1}\, dx\\[6pt]
\text{Sustituyendo: } &u = e^{x} 
\;\;\Rightarrow\; du = e^{x}\, dx\\[6pt]
\int 1 - \frac{2}{e^{x} + 1}\, dx
&= x - 2\int \frac{1}{u \left(u + 1\right)} \, du \\[6pt]
&= x - 2\int \frac{1}{\left(\frac{1}{u} + 1\right) u^{2}} \, du \\[6pt]
\text{Sustituyendo: } &v = \frac{1}{u} + 1
\;\;\Rightarrow\; dv = -\frac{1}{u^{2}}\, du\\[6pt]
x+ 2\int \frac{1}{\left(\frac{1}{u} + 1\right) u^{2}} \, du
&= x + 2\int \frac{1}{v} \, dv \\[6pt]
&= x+2\ln\left|v\right|\\[6pt]
&= x+2\ln\left|\frac{1}{e^{x}}+1\right|+ C\\[6pt]
&= x+2\ln\left|\frac{1+e^{x}}{e^{x}}\right|+ C\\[6pt]
&= x+2\ln\left(1+e^{x}\right)- 2 \ln\left(e^{x}\right)+ C\\[6pt]
&= 2\ln\left(1+e^{x}\right)- x + C\\[6pt]
\end{align*}
\[
\boxed{\displaystyle \int
    \frac{e^{x} - 1}{e^{x} + 1}\,dx 
    = 2 \ln\left(1+e^{x}\right)- x + C\\[6pt]
}
\]  