$\displaystyle \mathbf{ \int 
        \frac{ln^{2}x + 2}{x \left(1 - ln x \right)}
    \,dx}$ 
\nopagebreak
\begin{align*}
\int \frac{\ln^{2}x + 2}{x \left(1 - \ln x \right)}\, dx
&= -\int \frac{\ln^{2}x + 2}{x \left(\ln x - 1\right)}\, dx \\[6pt]
\text{Sustituyendo: } &u = \ln x -1
\;\;\Rightarrow\; du = \frac{dx}{x}
\;\;\Rightarrow\; \ln^{2}x = \left(u+1\right)^{2} \\[6pt]
\int \frac{\ln^{2}x + 2}{x \left(1 - \ln x \right)}\, dx
&= -\int \frac{\left(u + 1\right)^{2} + 2}{u} \, du\\[6pt]
&= -\int u + \frac{3}{u} + 2\, du \\[6pt]
&= -3 \ln u - \frac{u^{2}}{2} - 2u \\[6pt]
&= -3 \ln\left|\ln x - 1\right| - 2 \left(\ln x - 1\right) - \frac{\left(\ln x - 1\right)^{2}}{2} + C \\[6pt]
&= -3 \ln\left|\ln x - 1\right| - \frac{1}{2} \ln x \left(\ln x + 2\right) + C
\end{align*}
\[
\boxed{\displaystyle \int
    \frac{\ln^{2}x + 2}{x \left(1 - \ln x \right)}
    \,dx 
    = -3 \ln\left|\ln x - 1\right| - \frac{1}{2} \ln x \left(\ln x + 2\right) + C
}
\]  